Refactored some code for proc+mem impl.

Kami/Ex/ProcMemOk.v
@@ -1,8 +1,11 @@
 Require Import Kami.
 Require Import Lib.FinNotations Lib.Struct Lib.Indexer.
-Require Import Ex.OneEltFifo Ex.ProcMemSpec Ex.PipelinedProc Ex.DecExec.
+Require Import Ex.OneEltFifo Ex.ProcMemSpec Ex.PipelinedProc
+        Ex.DecExec Ex.DecExecOk Ex.ProcMemInterm.
 
 Require Import Kami.Tactics Kami.ModuleBoundEx.
+
+Set Implicit Arguments.
 
 Section PipelinedProc.
   Variables (instK dataK: Kind)
@@ -13,78 +16,17 @@ Section PipelinedProc.
             (exec: Executer dataK).
 
   Variable (init: ProcInit instK dataK rfSize pgmSize).
-  
-  Definition procImpl2 :=
-    ((decexec dec exec (pcInit init) (pgmInit init))
-       ++ (regFile (rfInit init))
-       ++ (e2w dataK rfSize)
-       ++ (scoreboard rfSize)
-       ++ (writeback dataK rfSize))%kami.
-  Lemma procImpl2_PhoasWf: ModPhoasWf procImpl2.
-  Proof. kequiv. Qed.
-  Lemma procImpl2_RegsWf: ModRegsWf procImpl2.
-  Proof. kvr. Qed.
-  Hint Resolve procImpl2_PhoasWf procImpl2_RegsWf.
 
-  Hint Unfold procImpl2: ModuleDefs.
-  
-  Theorem procImpl_ok_1:
-    procImpl dec exec init <<== procImpl2.
-  Proof.
-    kmodular.
-    - apply decexec_ok.
-    - krefl.
-  Qed.
-
+  Local Notation procIntermInl := (procIntermInl dec exec init).
   Local Notation RfWrite := (RfWrite dataK rfSize).
 
-  Definition procImpl2_regMap (r: RegsT): RegsT :=
-    (mlet pcv: (Bit pgmSize) <- r |> "pc";
-       mlet pgmv: (Vector instK pgmSize) <- r |> "pgm";
-       mlet rfv: (Vector dataK rfSize) <- r |> "rf";
-       mlet e2wfullv: Bool <- r |> "e2w"--"full";
-       mlet e2weltv: (Struct RfWrite) <- r |> "e2w"--"elt";
-       mlet sbFlagsv: (Vector Bool rfSize) <- r |> "sbFlags";
-       (["pgm" <- existT _ _ pgmv]
-        +["rf" <- existT _ _
-               (if e2wfullv
-                then evalExpr (#rfv@[#e2weltv!RfWrite@."idx"
-                               <- #e2weltv!RfWrite@."val"])%kami_expr
-                else rfv)]
-        +["pc" <- existT _ _ pcv])%fmap)%mapping.
-  Hint Unfold procImpl2_regMap: MapDefs.
-
-  Definition procImpl2_ruleMap (o: RegsT): string -> option string :=
-    "decexecArith" |-> "doArith";
-      "decexecLd" |-> "doLoad";
-      "decexecSt" |-> "doStore";
-      "decexecTh" |-> "doToHost"; ||.
-  Hint Unfold procImpl2_ruleMap: MethDefs.
-
-  Definition procImpl2Inl: sigT (fun m: Modules => procImpl2 <<== m).
-  Proof.
-    pose proof (inlineF_refines
-                  (procImpl2_PhoasWf type typeUT)
-                  (Reflection.noDupStr_NoDup
-                     (namesOf (getDefsBodies procImpl2))
-                     eq_refl)) as Him.
-    unfold MethsT in Him; rewrite <-SemFacts.idElementwiseId in Him.
-    match goal with
-    | [H: context[inlineF ?m] |- _] => set m as origm in H at 2
-    end.
-    kinline_compute_in Him.
-    unfold origm in *.
-    specialize (Him eq_refl).
-    exact (existT _ _ Him).
-  Defined.
-
-  Definition procImpl2_scoreboard_inv
+  Definition procInterm_scoreboard_inv
              (sbFlagsv: fullType type (SyntaxKind (Vector Bool rfSize)))
              (e2wfullv: fullType type (SyntaxKind Bool))
              (e2weltv: fullType type (SyntaxKind (Struct RfWrite))) :=
     e2wfullv = true -> sbFlagsv (e2weltv F1) = true.
 
-  Record procImpl2_inv (o: RegsT): Prop :=
+  Record procInterm_inv (o: RegsT): Prop :=
     { pcv: fullType type (SyntaxKind (Bit pgmSize));
       Hpcv: M.find "pc"%string o = Some (existT _ _ pcv);
       pgmv: fullType type (SyntaxKind (Vector instK pgmSize));
@@ -98,71 +40,95 @@ Section PipelinedProc.
       sbFlagsv: fullType type (SyntaxKind (Vector Bool rfSize));
       HsbFlagsv: M.find "sbFlags"%string o = Some (existT _ _ sbFlagsv);
 
-      HsbInv: procImpl2_scoreboard_inv sbFlagsv e2wfullv e2weltv;
+      HsbInv: procInterm_scoreboard_inv sbFlagsv e2wfullv e2weltv;
     }.
-  Hint Unfold procImpl2_scoreboard_inv : InvDefs.
+  Hint Unfold procInterm_scoreboard_inv : InvDefs.
 
-  Ltac procImpl2_inv_dest_tac :=
+  Ltac procInterm_inv_dest_tac :=
     try match goal with
-        | [H: procImpl2_inv _ |- _] => destruct H
+        | [H: procInterm_inv _ |- _] => destruct H
         end;
     kinv_red.
 
-  Ltac procImpl2_inv_constr_tac :=
+  Ltac procInterm_inv_constr_tac :=
     econstructor;
     repeat (intros; try findReify;
             kinv_eq; kinv_red; eauto).
 
-  Ltac procImpl2_inv_tac :=
-    procImpl2_inv_dest_tac; procImpl2_inv_constr_tac.
+  Ltac procInterm_inv_tac :=
+    procInterm_inv_dest_tac; procInterm_inv_constr_tac.
 
-  Lemma procImpl2_inv_ok':
+  Lemma procInterm_inv_ok':
     forall init n ll,
-      init = initRegs (getRegInits (projT1 procImpl2Inl)) ->
-      Multistep (projT1 procImpl2Inl) init n ll ->
-      procImpl2_inv n.
+      init = initRegs (getRegInits (projT1 procIntermInl)) ->
+      Multistep (projT1 procIntermInl) init n ll ->
+      procInterm_inv n.
   Proof.
     induction 2.
-    - unfold getRegInits, procImpl2Inl, projT1.
-      procImpl2_inv_tac; simpl in *; kinv_simpl.
+    - unfold getRegInits, procIntermInl, projT1.
+      procInterm_inv_tac; simpl in *; kinv_simpl.
     - kinvert.
       + mred.
       + mred.
-      + kinv_dest_custom procImpl2_inv_tac.
-      + kinv_dest_custom procImpl2_inv_tac.
-      + kinv_dest_custom procImpl2_inv_tac.
-      + kinv_dest_custom procImpl2_inv_tac.
-      + kinv_dest_custom procImpl2_inv_tac.
+      + kinv_dest_custom procInterm_inv_tac.
+      + kinv_dest_custom procInterm_inv_tac.
+      + kinv_dest_custom procInterm_inv_tac.
+      + kinv_dest_custom procInterm_inv_tac.
+      + kinv_dest_custom procInterm_inv_tac.
   Qed.
 
-  Lemma procImpl2_inv_ok:
+  Lemma procInterm_inv_ok:
     forall o,
-      reachable o (projT1 procImpl2Inl) ->
-      procImpl2_inv o.
+      reachable o (projT1 procIntermInl) ->
+      procInterm_inv o.
   Proof.
     intros; inv H; inv H0.
-    eapply procImpl2_inv_ok'; eauto.
+    eapply procInterm_inv_ok'; eauto.
   Qed.
 
-  Theorem procImpl_ok_2: procImpl2 <<== procSpec dec exec init.
+  Definition procInterm_regMap (r: RegsT): RegsT :=
+    (mlet pcv: (Bit pgmSize) <- r |> "pc";
+       mlet pgmv: (Vector instK pgmSize) <- r |> "pgm";
+       mlet rfv: (Vector dataK rfSize) <- r |> "rf";
+       mlet e2wfullv: Bool <- r |> "e2w"--"full";
+       mlet e2weltv: (Struct RfWrite) <- r |> "e2w"--"elt";
+       mlet sbFlagsv: (Vector Bool rfSize) <- r |> "sbFlags";
+       (["pgm" <- existT _ _ pgmv]
+        +["rf" <- existT _ _
+               (if e2wfullv
+                then evalExpr (#rfv@[#e2weltv!RfWrite@."idx"
+                               <- #e2weltv!RfWrite@."val"])%kami_expr
+                else rfv)]
+        +["pc" <- existT _ _ pcv])%fmap)%mapping.
+  Hint Unfold procInterm_regMap: MapDefs.
+
+  Definition procInterm_ruleMap (o: RegsT): string -> option string :=
+    "decexecArith" |-> "doArith";
+      "decexecLd" |-> "doLoad";
+      "decexecSt" |-> "doStore";
+      "decexecTh" |-> "doToHost"; ||.
+  Hint Unfold procInterm_ruleMap: MethDefs.
+
+  Theorem procImpl_ok_2:
+    procInterm dec exec init <<== procSpec dec exec init.
   Proof.
     intros.
 
     (* 1) inlining *)
-    ketrans; [exact (projT2 procImpl2Inl)|].
+    ketrans; [exact (projT2 procIntermInl)|].
 
     (* 2) decomposition *)
-    kdecompose_nodefs procImpl2_regMap procImpl2_ruleMap.
+    kdecompose_nodefs procInterm_regMap procInterm_ruleMap.
 
     (* (* 3) simulation *) *)
-    kinv_add procImpl2_inv_ok.
+    kinv_add procInterm_inv_ok.
     kinv_add_end.
     kinvert.
-    - kinv_magic_with procImpl2_inv_tac idtac.
-    - kinv_magic_with procImpl2_inv_tac idtac.
-    - kinv_magic_with procImpl2_inv_tac idtac.
-    - kinv_magic_with procImpl2_inv_tac idtac.
-    - kinv_magic_with procImpl2_inv_tac idtac.
+    - kinv_magic_with procInterm_inv_tac idtac.
+    - kinv_magic_with procInterm_inv_tac idtac.
+    - kinv_magic_with procInterm_inv_tac idtac.
+    - kinv_magic_with procInterm_inv_tac idtac.
+    - kinv_magic_with procInterm_inv_tac idtac.
   Qed.
 
   Theorem procImpl_ok:
