Kami/Ex/DecExecOk.v
@@ -1,0 +1,131 @@
+Require Import Kami.
+Require Import Lib.FinNotations Lib.Struct Lib.Indexer.
+Require Import Ex.ProcMemSpec Ex.PipelinedProc Ex.DecExec.
+
+Set Implicit Arguments.
+
+Section DecExec.
+  Variables (instK dataK: Kind)
+            (addrSize rfSize: nat)
+            (pgmSize: nat).
+
+  Variables (dec: Decoder instK addrSize rfSize)
+            (exec: Executer dataK)
+            (pcInit : ConstT (Bit pgmSize))
+            (pgmInit : ConstT (Vector instK pgmSize)).
+
+  Local Notation D2E := (D2E addrSize rfSize pgmSize).
+  Local Notation decexecSepInl := (decexecSepInl dec exec pcInit pgmInit).
+
+  Definition decexec_regMap (r: RegsT): RegsT :=
+    (mlet pcv : (Bit pgmSize) <- r |> "pc";
+     mlet pgmv : (Vector instK pgmSize) <- r |> "pgm";
+     mlet d2efullv : Bool <- r |> "d2e"--"full";
+     mlet d2eeltv : (Struct D2E) <- r |> "d2e"--"elt";
+     (["pgm" <- existT _ _ pgmv]
+      +["pc" <- existT _ (SyntaxKind (Bit pgmSize))
+             (if d2efullv then d2eeltv F7 else pcv)])%fmap)%mapping.
+  Hint Unfold decexec_regMap: MapDefs.
+  
+  Definition decexec_ruleMap (o: RegsT): string -> option string :=
+    "executeArith" |-> "decexecArith";
+      "executeLd" |-> "decexecLd";
+      "executeSt" |-> "decexecSt";
+      "executeTh" |-> "decexecTh"; ||.
+  Hint Unfold decexec_ruleMap: MethDefs.
+
+  Definition decexec_d2e_inv
+             (pgmv: fullType type (SyntaxKind (Vector instK pgmSize)))
+             (d2efullv: fullType type (SyntaxKind Bool))
+             (d2eeltv: fullType type (SyntaxKind (Struct D2E))) :=
+    d2efullv = true ->
+    let pc := d2eeltv F7 in
+    let inst := evalExpr (#pgmv@[#pc])%kami_expr in
+    d2eeltv F1 = evalExpr (getOp dec inst) /\
+    d2eeltv F2 = evalExpr (getArithOp dec inst) /\
+    d2eeltv F3 = evalExpr (getSrc1 dec inst) /\
+    d2eeltv F4 = evalExpr (getSrc2 dec inst) /\
+    d2eeltv F5 = evalExpr (getDst dec inst) /\
+    d2eeltv F6 = evalExpr (getAddr dec inst).
+
+  Record decexec_inv (o: RegsT): Prop :=
+    { pcv: fullType type (SyntaxKind (Bit pgmSize));
+      Hpcv: M.find "pc"%string o = Some (existT _ _ pcv);
+      pgmv: fullType type (SyntaxKind (Vector instK pgmSize));
+      Hpgmv: M.find "pgm"%string o = Some (existT _ _ pgmv);
+      d2efullv: fullType type (SyntaxKind Bool);
+      Hd2efullv: M.find "full.d2e"%string o = Some (existT _ _ d2efullv);
+      d2eeltv: fullType type (SyntaxKind (Struct D2E));
+      Hd2eeltv: M.find "elt.d2e"%string o = Some (existT _ _ d2eeltv);
+
+      Hpcinv: d2efullv = true -> pcv = d2eeltv F7 ^+ $1;
+      Hdeinv: decexec_d2e_inv pgmv d2efullv d2eeltv
+    }.
+  Hint Unfold decexec_d2e_inv : InvDefs.
+
+  Ltac decexec_inv_dest_tac :=
+    try match goal with
+    | [H: decexec_inv _ |- _] => destruct H
+    end;
+    kinv_red.
+
+  Ltac decexec_inv_constr_tac :=
+    econstructor;
+    repeat (intros; try findReify;
+            kinv_eq; kinv_red; eauto).
+
+  Ltac decexec_inv_tac :=
+    decexec_inv_dest_tac; decexec_inv_constr_tac.
+
+  Lemma decexec_inv_ok':
+    forall init n ll,
+      init = initRegs (getRegInits (projT1 decexecSepInl)) ->
+      Multistep (projT1 decexecSepInl) init n ll ->
+      decexec_inv n.
+  Proof.
+    induction 2.
+    - unfold getRegInits, decexecSepInl, projT1.
+      decexec_inv_tac; simpl in *; kinv_simpl.
+    - kinvert.
+      + mred.
+      + mred.
+      + kinv_dest_custom decexec_inv_tac.
+      + kinv_dest_custom decexec_inv_tac.
+      + kinv_dest_custom decexec_inv_tac.
+      + kinv_dest_custom decexec_inv_tac.
+      + kinv_dest_custom decexec_inv_tac.
+  Qed.
+
+  Lemma decexec_inv_ok:
+    forall o,
+      reachable o (projT1 decexecSepInl) ->
+      decexec_inv o.
+  Proof.
+    intros; inv H; inv H0.
+    eapply decexec_inv_ok'; eauto.
+  Qed.
+  
+  Theorem decexec_ok:
+    decexecSep dec exec pcInit pgmInit <<== decexec dec exec pcInit pgmInit.
+  Proof.
+    intros.
+
+    (* 1) inlining *)
+    ketrans; [exact (projT2 decexecSepInl)|].
+
+    (* 2) decomposition *)
+    kdecompose_nodefs decexec_regMap decexec_ruleMap.
+
+    (* 3) simulation *)
+    kinv_add decexec_inv_ok.
+    kinv_add_end.
+    kinvert.
+    - kinv_magic_with decexec_inv_dest_tac idtac.
+    - kinv_magic_with decexec_inv_dest_tac idtac.
+    - kinv_magic_with decexec_inv_dest_tac idtac.
+    - kinv_magic_with decexec_inv_dest_tac idtac.
+    - kinv_magic_with decexec_inv_dest_tac idtac.
+  Qed.
+  
+End DecExec.
+
