Kami/Ex/ProcMemInterm.v
@@ -1,0 +1,60 @@
+Require Import Kami.
+Require Import Lib.FinNotations Lib.Struct Lib.Indexer.
+Require Import Ex.OneEltFifo Ex.ProcMemSpec Ex.PipelinedProc
+        Ex.DecExec Ex.DecExecOk.
+
+Require Import Kami.Tactics Kami.ModuleBoundEx.
+
+Set Implicit Arguments.
+
+Section PipelinedProc.
+  Variables (instK dataK: Kind)
+            (addrSize rfSize: nat)
+            (pgmSize: nat).
+
+  Variables (dec: Decoder instK addrSize rfSize)
+            (exec: Executer dataK).
+
+  Variable (init: ProcInit instK dataK rfSize pgmSize).
+  
+  Definition procInterm :=
+    ((decexec dec exec (pcInit init) (pgmInit init))
+       ++ (regFile (rfInit init))
+       ++ (e2w dataK rfSize)
+       ++ (scoreboard rfSize)
+       ++ (writeback dataK rfSize))%kami.
+  Lemma procInterm_PhoasWf: ModPhoasWf procInterm.
+  Proof. kequiv. Qed.
+  Lemma procInterm_RegsWf: ModRegsWf procInterm.
+  Proof. kvr. Qed.
+  Hint Resolve procInterm_PhoasWf procInterm_RegsWf.
+
+  Hint Unfold procInterm: ModuleDefs.
+  
+  Theorem procImpl_ok_1:
+    procImpl dec exec init <<== procInterm.
+  Proof.
+    kmodular.
+    - apply decexec_ok.
+    - krefl.
+  Qed.
+
+  Definition procIntermInl: sigT (fun m: Modules => procInterm <<== m).
+  Proof.
+    pose proof (inlineF_refines
+                  (procInterm_PhoasWf type typeUT)
+                  (Reflection.noDupStr_NoDup
+                     (namesOf (getDefsBodies procInterm))
+                     eq_refl)) as Him.
+    unfold MethsT in Him; rewrite <-SemFacts.idElementwiseId in Him.
+    match goal with
+    | [H: context[inlineF ?m] |- _] => set m as origm in H at 2
+    end.
+    kinline_compute_in Him.
+    unfold origm in *.
+    specialize (Him eq_refl).
+    exact (existT _ _ Him).
+  Defined.
+
+End PipelinedProc.
+
